FOL/NV/Sub/Var/All/Rec/Admits.lean
@@ -74,7 +74,7 @@ instance
 theorem substitution_theorem_aux
   (D : Type)
   (I : Interpretation D)
-  (V V' : Assignment D)
+  (V V' : Valuation_ D)
   (E : Env)
   (σ σ' : VarName → VarName)
   (binders : Finset VarName)
@@ -209,7 +209,7 @@ theorem substitution_theorem_aux
 theorem substitution_theorem
   (D : Type)
   (I : Interpretation D)
-  (V : Assignment D)
+  (V : Valuation_ D)
   (E : Env)
   (σ : VarName → VarName)
   (F : Formula)
